extraction/extraction.v
@@ -199,7 +199,7 @@ Cd "extraction".
 
 Separate Extraction
    Compiler.transf_c_program Compiler.transf_cminor_program
-   Compiler.transf_c_program_bytes
+   Compiler.transf_c_program_assembler
    Cexec.do_initial_state Cexec.do_step Cexec.at_final_state
    Ctypes.merge_attributes Ctypes.remove_attributes Ctypes.build_composite_env
    Initializers.transl_init Initializers.constval
